Tag HOL set_var/upd_locals/empty_locals over CrepHolState

scripts/hol-probes/crep_local_updates_probeScript.sml
@@ -1,0 +1,49 @@
+(*
+  Direct HOL observations for crepSem$set_var_def / upd_locals_def /
+  empty_locals_def.
+  Reference: cakeml/pancake/semantics/crepSemScript.sml:55-73.
+*)
+load "bossLib";
+load "preamble";
+load "crepSemTheory";
+open bossLib;
+open HolKernel Parse;
+open preamble;
+open crepSemTheory;
+
+val s = ``(s:(8,unit) crepSem$state)``;
+val s0 = ``(^s with <|locals := FEMPTY |+ (2, Word (9w:8 word));
+                       clock := 5; base_addr := 3w; top_addr := 100w|>)``;
+
+fun print_eval label q =
+  let
+    val th = EVAL q
+  in
+    print (label ^ "=");
+    print_term (rconc th);
+    print "\n"
+  end;
+
+val _ = print_eval "set_var_hit"
+  ``FLOOKUP ((crepSem$set_var 1 (Word (7w:8 word)) (^s0)).locals) 1 =
+      SOME (Word (7w:8 word))``;
+
+val _ = print_eval "set_var_keeps_other"
+  ``FLOOKUP ((crepSem$set_var 1 (Word (7w:8 word)) (^s0)).locals) 2 =
+      SOME (Word (9w:8 word))``;
+
+val _ = print_eval "upd_locals_replace"
+  ``(case crepSem$upd_locals [(1,(Word (3w:8 word)))] (^s0) of s' =>
+      (FLOOKUP s'.locals 1 = SOME (Word (3w:8 word))) /\
+      (FLOOKUP s'.locals 2 = NONE))``;
+
+val _ = print_eval "empty_locals_none"
+  ``FLOOKUP ((crepSem$empty_locals (^s0)).locals) 2 = NONE``;
+
+val _ = print_eval "set_var_fields_preserved"
+  ``(case crepSem$set_var 1 (Word (7w:8 word)) (^s0) of s' =>
+      (s'.clock = 5) /\ (s'.base_addr = 3w) /\ (s'.top_addr = 100w))``;
+
+val _ = print_eval "empty_locals_fields_preserved"
+  ``(case crepSem$empty_locals (^s0) of s' =>
+      (s'.clock = 5) /\ (s'.memory = (^s0).memory))``;
